Start verifying the real Go WaitGroup implementation,
rather than using a trusted mode; starting to do so helped clean up/fix a
bunch of little things in Goose and the go proof library.

Unlike `Mutex`, `WaitGroup` doesn't have any data races. Goose can now
translate WaitGroup and its methods, and a proof seems doable. The hard
part in the proof is that WaitGroup treats a 64-bit word as logically
storing two different 32-bit pieces of state. A mini abstraction for
handling this "two 32-bit words as a 64-bit word" pattern would probably
simplify/hide the convoluted word proofs that are currently dealing with
bit operations.

Added a trusted impl for a bit of `sync/atomic`, and verified
other parts of it, since `waitgroup.go` uses it. Also added a
simple trusted model for `runtime_Semacquire` based on
`runtime/sema.go`.

new/etc/update-goose-new.py
@@ -204,7 +204,11 @@ def main():
         "slices",
         "strconv",
         "strings",
+
         "sync",
+        "sync/atomic",
+        "internal/race",
+
         "fmt",
         "log",
         "go.etcd.io/raft/v3/raftpb",
