new/golang/theory/builtin.v
@@ -1,5 +1,6 @@
 From New Require Export notation.
-From New.golang.theory Require Export typing.
+From New.golang.defn Require Export builtin.
+From New.golang.theory Require Export typing proofmode.
 
 Module error.
   Section def.
@@ -7,3 +8,21 @@ Module error.
   Definition t := interface.t.
   End def.
 End error.
+
+Section wps.
+
+Context `{sem: ffi_semantics} `{!ffi_interp ffi} `{!heapGS Σ}.
+
+Global Instance wp_int64_gt (l r : w64) : PureWp True (int_gt #l #r) #(bool_decide (sint.Z l > sint.Z r)).
+Proof. Admitted.
+
+Global Instance wp_int64_lt (l r : w64) : PureWp True (int_lt #l #r) #(bool_decide (sint.Z l < sint.Z r)).
+Proof. Admitted.
+
+Global Instance wp_int32_gt (l r : w32) : PureWp True (int_gt #l #r) #(bool_decide (sint.Z l > sint.Z r)).
+Proof. Admitted.
+
+Global Instance wp_int32_lt (l r : w32) : PureWp True (int_lt #l #r) #(bool_decide (sint.Z l < sint.Z r)).
+Proof. Admitted.
+
+End wps.
