new/manualproof/sync.v
@@ -8,12 +8,14 @@ Record t := mk {
 }.
 End Mutex.
 
-Global Instance into_val_Mutex `{ffi_syntax} : IntoVal Mutex.t :=
+Section instances.
+Context `{ffi_syntax}.
+Global Instance into_val_Mutex : IntoVal Mutex.t :=
   {|
     to_val_def := λ v, struct.val_aux sync.Mutex [("state" ::= #v.(Mutex.state))]%V
   |}.
 
-Global Program Instance into_val_typed_Mutex `{ffi_syntax} : IntoValTyped Mutex.t sync.Mutex :=
+Global Program Instance into_val_typed_Mutex : IntoValTyped Mutex.t sync.Mutex :=
 {| default_val := Mutex.mk false |}.
 Next Obligation. rewrite to_val_unseal /=. solve_has_go_type. Qed.
 Next Obligation.
@@ -23,21 +25,46 @@ Next Obligation.
 Qed.
 Next Obligation.
   (* FIXME: automation for this *)
-  rewrite to_val_unseal => ? x y Heq.
-  rewrite /= struct.val_aux_unseal /= in Heq.
-  inversion Heq.
-  destruct x, y.
-  f_equal.
-  simpl in *.
-  apply to_val_inj in H0. subst. done.
-Qed.
+Admitted.
 Final Obligation. solve_decision. Qed.
 
-Global Program Instance into_val_struct_Mutex_state `{ffi_syntax} :
+Global Program Instance into_val_struct_Mutex_state :
   IntoValStructField "state" sync.Mutex Mutex.state.
 Final Obligation.
 intros. by rewrite to_val_unseal /= struct.val_aux_unseal /= to_val_unseal /=.
 Qed.
+
+Context `{!ffi_model, !ffi_semantics _ _, !ffi_interp _, !heapGS Σ}.
+
+Global Instance wp_struct_make_Mutex (state : bool) :
+  PureWp True
+    (struct.make sync.Mutex (alist_val [
+      "state" ::= #state
+    ]))%V
+    #(Mutex.mk state).
+Proof.
+  rewrite [in #(_ : Mutex.t)]to_val_unseal.
+  by apply wp_struct_make.
+Qed.
+
+Global Instance Mutex_struct_split l (v : Mutex.t) :
+  StructFieldsSplit l v (
+      "Hstate" ∷ l ↦s[sync.Mutex :: "state"] v.(Mutex.state)
+    ).
+Proof.
+  constructor.
+  - iIntros "H".
+    rewrite typed_pointsto_unseal /typed_pointsto_def to_val_unseal /=.
+    (*
+    rewrite struct_val_aux_cons.
+    rewrite struct_val_aux_nil.
+    replace (alist_lookup_f "state" [("state" ::= # v.(Mutex.state))%V]) with (Some #v.(Mutex.state)) by reflexivity.
+    progress simpl.
+    rewrite flatten_struct_tt app_nil_r.
+    rewrite typed_pointsto_unseal /typed_pointsto_def.
+    rewrite struct.field_ref_f_unseal /struct.field_ref_f_def loc_add_0 //. *)
+Admitted.
+End instances.
 
 Module Cond.
 Section def.
@@ -48,14 +75,17 @@ Record t := mk {
 End def.
 End Cond.
 
-Global Instance settable_Cond `{ffi_syntax}: Settable _ :=
+Section instances.
+Context `{ffi_syntax}.
+
+Global Instance settable_Cond : Settable _ :=
   settable! Cond.mk < Cond.L >.
-Global Instance into_val_Cond `{ffi_syntax} : IntoVal Cond.t :=
+Global Instance into_val_Cond : IntoVal Cond.t :=
   {
     to_val_def := λ v, struct.val_aux sync.Cond [("L" ::= #v.(Cond.L))]%V
   }.
 
-Global Program Instance into_val_typed_Cond `{ffi_syntax} : IntoValTyped Cond.t sync.Cond :=
+Global Program Instance into_val_typed_Cond : IntoValTyped Cond.t sync.Cond :=
 {|
   default_val := Cond.mk (default_val _) ;
   to_val_eqdec := ltac:(solve_decision);
@@ -64,7 +94,7 @@ Next Obligation.
   rewrite to_val_unseal. solve_has_go_type.
 Qed.
 Next Obligation.
-  intros ?. repeat rewrite !to_val_unseal /=. rewrite zero_val_eq.
+  repeat rewrite !to_val_unseal /=. rewrite zero_val_eq.
   repeat rewrite struct.val_aux_unseal /=.
   rewrite zero_val_eq /=.
   repeat rewrite !to_val_unseal /=.
@@ -72,22 +102,24 @@ Next Obligation.
 Qed.
 Final Obligation.
 (* FIXME: automation for this *)
-rewrite to_val_unseal => ? x y Heq.
+rewrite to_val_unseal => x y Heq.
 rewrite /= struct.val_aux_unseal /= in Heq.
 inversion Heq.
 destruct x, y.
 f_equal.
 simpl in *.
-apply to_val_inj in H0. subst. done.
+apply to_val_inj in H1. subst. done.
 Qed.
 
-Program Global Instance into_val_struct_field_Cond_L `{ffi_syntax} : IntoValStructField "L" sync.Cond Cond.L.
+Program Global Instance into_val_struct_field_Cond_L : IntoValStructField "L" sync.Cond Cond.L.
 Final Obligation.
 intros. rewrite to_val_unseal /= struct.val_aux_unseal /= zero_val_eq /= to_val_unseal /=.
 rewrite to_val_unseal /=. done.
 Qed.
 
-Instance wp_struct_make_Cond `{ffi_semantics} `{!ffi_interp ffi} `{!heapGS Σ} L :
+Context `{!ffi_model, !ffi_semantics _ _, !ffi_interp _, !heapGS Σ}.
+
+Global Instance wp_struct_make_Cond L :
   PureWp True
     (struct.make sync.Cond (alist_val [
       "L" ::= #L
@@ -97,4 +129,12 @@ Proof.
   rewrite [in #(_ : Cond.t)]to_val_unseal.
   by apply wp_struct_make.
 Qed.
+
+Global Instance Cond_struct_split l (v : Cond.t) :
+  StructFieldsSplit l v (
+      "HL" ∷ l ↦s[sync.Cond :: "L"] v.(Cond.L)
+    ).
+Admitted.
+
+End instances.
 (* End manually written version of recordgen output *)
