new/proof/etcdraft.v
@@ -6,11 +6,4 @@ From New.proof Require Import grove_prelude.
 Section proof.
 Context `{!heapGS Σ}.
 
-(* FIXME: move to builtin *)
-Instance wp_int_gt (l r : w64) : PureWp True (int_gt #l #r) #(bool_decide (sint.Z l > sint.Z r)).
-Proof. Admitted.
-
-Instance wp_int_lt (l r : w64) : PureWp True (int_lt #l #r) #(bool_decide (sint.Z l < sint.Z r)).
-Proof. Admitted.
-
 End proof.
