new/trusted_code/sync/atomic.v
@@ -1,0 +1,17 @@
+From New.golang Require Import defn.
+
+Module atomic.
+Section code.
+Context `{ffi_syntax}.
+
+Definition LoadUint64 : val :=
+  λ: "addr", Load "addr".
+
+Definition StoreUint64 : val :=
+  λ: "addr" "val", AtomicStore "addr" "val".
+
+Definition AddUint64 : val :=
+  λ: "addr", #() #().
+
+End code.
+End atomic.
